Evaluation.v
@@ -12,10 +12,9 @@ Require Import Util.
 
 Module Evaluation.
 
-  Export Graph.Graph NeList.NeList.
+  Export Graph.TCFG Graph.CFG NeList.NeList. 
 
   Parameter Val : Type.
-  Definition Tag := list nat.
 
   Definition State := Var -> Val.
 
@@ -27,7 +26,6 @@ Module Evaluation.
   Parameter start_tag : Tag.
 
   Definition States := State -> Prop.
-  Definition Coord := prod Lab Tag.
   Definition Conf := prod Coord State.
 
   Hint Unfold Conf Coord.
@@ -39,46 +37,25 @@ Module Evaluation.
 
   Parameter eff' : Lab * State -> option (Lab * State).
   
-  Fixpoint eff_tag (k : Conf) : Tag
-    := match k with
-         (p, i, s)
-         => match eff' (p,s) with
-             Some (q , r)
-             => if is_back_edge p q
-               then match i with
-                    | nil => nil
-                    | n :: l => (S n) :: l
-                    end
-               else 
-                    let l' := @iter Tag (@tl nat) i (length (loop_exit p)) in
-                    if loop_head_dec q then O :: l' else l'
-                |
-             None => nil
-           end
-       end.
-
   Definition eff (k : Conf) : option Conf
     := match k with
        | (p, i, s) => match eff' (p,s) with
                   | None => None
-                  | Some (q, r) => Some (q, eff_tag k, r)
+                  | Some (q, r) => Some (q, eff_tag p q i, r)
                   end
        end.
 
-    Lemma Conf_dec :
-    forall (x y : Conf), {x = y} + {x <> y}.
-  Proof.
+  Program Instance conf_eq_eqdec : EqDec Conf eq.
+  Next Obligation.
     intros.
     destruct x as [[p i] s], y as [[q j] r].
     destruct ((p, i, s) == (q, j, r)); firstorder.
   Qed.
-  Instance conf_eq_eqdec : EqDec Conf eq := Conf_dec.
-
-
-  Definition start_coord := (root, start_tag) : Coord.
+  Definition Conf_dec := conf_eq_eqdec.
 
   Definition is_effect_on (p q : Lab) :=
     exists i i' s s', eff ((p, i), s) = Some ((q, i'), s').
+  Parameter zero : State.
 
   Parameter edge_spec :
     forall p q, is_effect_on p q -> p --> q.
@@ -90,24 +67,87 @@ Module Evaluation.
     eapply edge_spec. 
     unfold is_effect_on. eauto.
   Qed.
+  
+  Program Instance EvalGraph : Graph Conf (start_coord,zero)
+                                     (fun k k' => match eff k return Prop with
+                                                 Some k => k = k' | None => False end).
+  Next Obligation.
+    destruct (eff p); [apply conf_eq_eqdec|tauto].
+  Qed.
+  Next Obligation.
+    intro N. destruct (eff p) eqn:E.
+    - subst c. destruct p,c. apply step_conf_implies_edge in E. apply root_no_pred' in E. assumption.
+    - contradiction.
+  Qed.
 
   Parameter def_spec :
     forall p q x, (exists i j s r, eff (p, i, s) = Some (q, j, r) /\ r x <> s x) ->
                   is_def x p q = true.
 
   Inductive Tr : ne_list Conf -> Prop :=
-    | Init : forall s, Tr (ne_single (root, start_tag, s))
-    | Step : forall l k, Tr l -> eff (ne_front l) = Some k -> Tr (k :<: l).
+  | Init : forall s, Tr (ne_single (root, start_tag, s))
+  | Step : forall l k, Tr l -> eff (ne_front l) = Some k -> Tr (k :<: l).
+
+  Definition EPath := @Path _ _ _ EvalGraph.
+
+  Ltac exploit' H :=
+    let p := fresh "Q" in
+           lazymatch type of H with
+           | ?P -> ?Q => assert P as p; [eauto|specialize (H p); clear p]
+           | forall (x : ?P), ?Q => assert P as p; [eauto|specialize (H p)]
+           end.
+
+  Ltac exploit H := repeat (exploit' H).
+  
+  Goal forall (V X Y Z : Type) (x:X) (y:Y) (P : V -> Prop), (X -> Y -> V) -> (forall v:V, P v -> X -> Y -> Z) -> (forall v, P v) -> Z.
+    intros V X Y Z x y P Hxy Hv HP. 
+    exploit Hxy. exploit Hv. exact Hv.
+  Qed.
+  
+  Lemma EPath_Tr s0 p i s π :
+    Path (root,start_tag,s0) (p,i,s) π -> Tr π.
+  Proof.
+    intro H. 
+    dependent induction H; [|destruct b,p0]; econstructor.
+    - eapply IHPath; eauto.
+    - erewrite path_front; eauto. destruct (eff (l,t,s1)); [subst c; eauto|contradiction].
+  Qed.
+
+  Lemma Tr_EPath p i s π :
+    (Tr π /\ ne_front π = (p,i,s)) -> exists s0, Path (root,start_tag,s0) (p,i,s) π.
+  Proof.
+    intros [HTr Hfront]. exists (snd (ne_back π)).
+    revert p i s Hfront. dependent induction HTr; cbn; intros p i s' Hfront.
+    - cbn in *. rewrite <-Hfront; econstructor.
+    - rewrite <-Hfront.
+      econstructor; [eapply IHHTr; eauto|].
+      + repeat rewrite <-surjective_pairing. reflexivity.
+      + replace (eff (_,_,_)) with (eff (ne_front l));
+          [|f_equal; repeat rewrite <-surjective_pairing; reflexivity].
+        destruct (eff _); inversion H; reflexivity.
+  Qed.
+
+  Lemma EPath_TPath k k' π :
+    EPath k k' π -> TPath (fst k) (fst k') (ne_map fst π).
+  Proof.
+    intros H. dependent induction H; [|destruct c]; econstructor.
+    - apply IHPath.
+    - repeat destr_let. destruct (eff _) eqn:E; [|contradiction]. split.
+      + subst c; eapply step_conf_implies_edge; eauto.
+      + unfold eff in E. destruct (eff' _) eqn:E'; [|congruence]. destruct p. destruct c,c.
+        inversion E. inversion H0. subst. reflexivity.
+  Qed.
 
   Ltac inv_dep H Dec := inversion H; subst; 
                         repeat match goal with
-                               | [ H0: @existT _ _ _ _ = @existT _ _ _ _  |- _ ] =>
-                                 apply inj_pair2_eq_dec in H0; try (apply Dec); subst
+                               | [ H0: @existT _ _ _ _ = @existT _ _ _ _  |- _ ]
+                                 => apply inj_pair2_eq_dec in H0; try (apply Dec); subst
                                end.
 
   Ltac inv_tr H := inversion H; subst; 
                    repeat match goal with
-                          | [ H0: @existT Conf _ _ _ = @existT _ _ _ _  |- _ ] => apply inj_pair2_eq_dec in H0; try (apply Conf_dec); subst
+                          | [ H0: @existT Conf _ _ _ = @existT _ _ _ _  |- _ ]
+                            => apply inj_pair2_eq_dec in H0; try (apply Conf_dec); subst
                           end.
 
   Definition trace := {l : ne_list Conf | Tr l}.
@@ -132,23 +172,6 @@ Module Evaluation.
     induction l; cbn in *; subst a; reflexivity.
   Qed.
 
-(*  Lemma tr_in_dec :
-    forall (k : Conf) t, {In k t} + {~ In k t}.
-  Proof.
-    intros k t. unfold In.
-    induction t; cbn in *.
-    - destruct (k == a); [left|right]; eauto.
-      intro H. destruct H as [H | [H | H]]; eauto. apply c. subst a. reflexivity. 
-    - inversion_clear IHt. 
-      + left. destruct H.
-        * right. right. apply ne_hd_hd in H. 
-          induction (ne_to_list t); cbn in *.
-          -- congruence.
-          -- left. inversion H. reflexivity.
-        * tauto.
-      + destruct (k == a); [left|right]; eauto. firstorder.
-  Qed.*)
-
   Lemma in_succ_in k p q t :
     Tr (nlcons k t) -> In p t -> eff p = Some q -> In q (k :: t).
   Proof.
@@ -156,19 +179,6 @@ Module Evaluation.
     revert dependent k. dependent induction t; intros k H; inv_tr H; try firstorder.
     + rewrite nlcons_front in H5. subst a. rewrite H5 in H1. inversion H1. left. reflexivity.
   Qed.
-
-(*  Lemma in_succ_exists p q i j s r t :
-    In (p, i, s) t (q, j, r) -> (exists k', eff (q, j, r) = Some k' /\ In (p, i, s) t k') \/ (p, i, s) = (q, j, r).
-  Proof.
-    intros Hin.
-    dependent induction t; inv_tr Hin; eauto.
-    destruct k' as [[a l] u].
-    left.
-    specialize (IHt a l u t).
-    destruct IHt; eauto.
-    + destruct H as [k' H]. exists k'. split; try constructor; firstorder.
-    + injection H; intros; subst. exists (p, i, s). firstorder. constructor.
-  Qed.*)
 
   Lemma in_pred_exists p i s k t :
     In (p,i,s) (k :<: t) ->
@@ -207,18 +217,6 @@ Module Evaluation.
   Definition Precedes' (l : list Conf) (k k' : Conf) : Prop :=
     exists l', Prefix (k' :: l') l /\ Precedes (k' :: l') k.
 
-(*  Definition PrecedesE (l : list Conf) (k k' : Conf) : Prop :=
-    exists l', Prefix (k' :: l') l /\ Precedes (k' :: l') k.*)
-  
-  
-(*  Inductive Precedes : forall k, Tr k -> Conf -> Conf -> Prop :=
-  | Pr_in : forall k t, Precedes k t k k
-  | Pr_cont : forall q q' p i j j' r' r s t step, Precedes (q', j', r') t (q, j, r) (q', j', r') -> 
-                                                  p =/= q ->
-                                                  Precedes (p, i, s) (Step (p, i, s) (q', j', r') t step) (q, j, r) (p, i, s)
-  | Pr_other : forall k' k t c c' step, Precedes k t c c' ->
-                                        Precedes k' (Step k' k t step) c c'.*)
-
   Lemma precedes_implies_in_pred k t :
     Precedes t k -> In k t.
   Proof.
@@ -228,174 +226,6 @@ Module Evaluation.
     - inv_tr H; eauto using In; cbn; eauto.
   Qed.
 
-(*  Lemma precedes_implies_in_succ k t k' k'' :
-    Precedes k t k' k'' -> In k t k''.
-  Proof.
-    intros H.
-    dependent induction t.
-    - inv_tr H. constructor.
-    - inv_tr H; eauto using In.
-  Qed.*)
-    
-(*  Lemma precedes_prefix k t c c' : 
-    Precedes k t c c' ->
-    exists tr, Prefix c' tr k t /\ Precedes c' tr c c'.
-  Proof.
-    intros Hprec.
-    dependent induction t.
-    + inv_tr Hprec.
-      - eexists. split; eauto using Prefix.
-    + inv_tr Hprec.
-      - eexists. split; constructor.
-      - eexists. split; [ constructor | eassumption ].
-      - eapply IHt in H4.
-        destruct H4 as [tr [Hprefix Hprec']].
-        exists tr. split; eauto using Prefix. 
-  Qed.
-
-  Lemma precedes_prefix_inv k t c c' l tr k' step : 
-    Precedes k' (Step k' k t step) c c' ->
-    Prefix k t l tr ->
-    forall l' step', Precedes l' (Step l' l tr step') c c'.
-  Proof.
-    intros Hprec Hprefix.
-    dependent induction Hprefix; intros l' step'.
-    + cut (Some k' = Some l'); intros.
-      - inject H.
-        cut (step = step'); intros; subst; try eassumption.
-        clear Hprec. destruct step'. apply UIP_refl.
-      - rewrite <- step. eassumption.
-    + constructor. eapply IHHprefix. eassumption.
-  Qed.
- *)
-  
-  (*Lemma in_prefix {A : Type} t (c : A) : 
-    In c t ->
-    exists pt, Prefix pt t /\
-          In c pt.
-  Proof.
-    intros.
-    dependent induction t.
-    + inv_tr H. exists (Init s). split; constructor.
-    + inv_tr H.
-    - exists tr0. split; constructor.
-    - eapply IHt in H4. destruct H4 as [pt [Hprefix Hin]].
-      exists pt. split; [ constructor | ]; eassumption.
-  Qed.
-  
-  Lemma in_prefix_in k t c k' t' :
-    In k t c ->
-    Prefix k t k' t' ->
-    In k' t' c.
-  Proof.
-    intros Hin Hprefix. dependent induction Hprefix; eauto using In.
-  Qed.*)
-
-(*  Fixpoint last_inst_of (l : Lab) (k : Conf) (t : trace) : option Tag :=
-    match t with
-    | (Init s) => if l == root then Some start_tag else None
-    | (Step (q, j, _) k t _) => if (l == q) then Some j else last_inst_of l k t
-    end.*)
-
-(*  Lemma last_inst_precedes_inv_helper q j r q' j' r' t e br m w :
-    Precedes (q, j, r) (Step (q, j, r) (q', j', r') t e)
-            (br, m, w) (q, j, r) ->
-    br =/= q ->
-    Precedes (q', j', r') t (br, m, w) (q', j', r').
-  Proof.
-    intros Hprec Hneq.
-    inv_tr Hprec.
-    - contradiction Hneq; reflexivity.
-    - eauto.
-    - exfalso. eapply (ivec_fresh _ _ _ _ _ step0); [ |reflexivity].
-      eauto using precedes_implies_in_succ. 
-  Qed.
-
-  Lemma last_inst_precedes_inv q j r br m w t : 
-    Precedes (q, j, r) t (br, m, w) (q, j, r) ->
-    last_inst_of br (q, j, r) t = Some m.
-  Proof.
-    intros Hprec.
-    dependent induction t; intros; simpl.
-    + destruct (br == root).
-      rewrite e in *. clear e.
-      inv_tr Hprec.
-      - reflexivity.
-      - inv_tr Hprec.
-        contradiction c; reflexivity.
-    + destruct k' as [[q' j'] r']. 
-      destruct (br == q).
-      * rewrite e0 in *. clear e0.
-        inv_tr Hprec; try reflexivity.
-        - contradiction H10; reflexivity.
-        - exfalso. eapply ivec_fresh. eapply step0.
-          eapply precedes_implies_in_succ. eassumption. reflexivity.
-      * eapply IHt; try reflexivity. 
-        eauto using last_inst_precedes_inv_helper.
-  Qed.
-
-  Lemma last_inst_precedes q j r br m t : 
-    last_inst_of br (q, j, r) t = Some m -> 
-    exists w, Precedes (q, j, r) t (br, m, w) (q, j, r).
-  Proof.
-    intros Hin.
-    dependent induction t; intros; simpl in Hin.
-    + destruct (br == root).
-      - rewrite e in *. clear e.
-        injection Hin; intros; subst.
-        exists r. constructor.
-      - inversion Hin.
-    + destruct k' as [[q' j'] r']. 
-      destruct (br == q).
-      * rewrite e0 in *. clear e0.
-        injection Hin; intros; subst; clear Hin.
-        exists r. constructor.
-      * eapply IHt in Hin; eauto.
-        destruct Hin as [w Hprec].
-        exists w. symmetry in c. eauto using Precedes.
-  Qed.
-
-(*  Definition unique_preceding q p :=
-      forall k k' t t' j j' i r r' s s',
-      Precedes k t (q, j, r) (p, i, s) ->
-      Precedes k' t' (q, j', r') (p, i, s') ->
-      j' = j.*)
-
-  Lemma path_for_trace k tr k' (Hin : In k tr k') :
-    { p: Path (lab_of k') (lab_of k) | forall q, PathIn q p -> exists j r, In k tr (q, j, r) }.
-  Proof.
-    destruct k as [[q j] r], k' as [[p i] s]. simpl.
-    dependent induction tr; intros.
-    + simpl.
-      enough (p = root).
-      - subst. exists (PathInit root). simpl. intros. rewrite H. eauto.
-      - inv_tr Hin; reflexivity.
-   + destruct k' as [[q' j'] r']; simpl in *.
-     destruct (p == q).
-     * rewrite e0. clear e0. exists (PathInit q). intros. 
-       inversion_clear H; subst. exists j, r. constructor.
-     * edestruct IHtr; eauto. inv_tr Hin.
-       - contradiction c; reflexivity.
-       - eapply H3.
-       - exists (PathStep p q' q x (step_conf_implies_edge q' q _ _ _ _ e)).
-         intros. simpl in H. inversion_clear H.
-         ++ rewrite H0. exists j, r. constructor.
-         ++ eapply e0 in H0. destruct H0 as [j0 [r0 H0]].
-            exists j0, r0. eauto using In.
-  Qed.
-
-  Lemma not_in_trace_exists_path (q : Lab) (k k' : Conf) (t : Tr k) (Hin : In k t k') : 
-    ~ (exists j r, In k t (q, j, r)) ->
-    ~ PathIn q (proj1_sig (path_for_trace k t k' Hin)).
-  Proof.
-    intros Hnin.
-    intro. apply Hnin. clear Hnin.
-    remember (path_for_trace k t k' Hin) as p.
-    clear Heqp.
-    destruct p as [p Hpin]; simpl in *.
-    eauto.
-  Qed.
-  *)
   Lemma start_no_tgt :
     forall i' s' k, eff k = Some (root, i', s') -> False.
   Proof.
@@ -404,7 +234,7 @@ Module Evaluation.
     unfold start_coord in H.
     cut (is_effect_on p root); intros.
     apply edge_spec in H0.
-    eapply root_no_pred. eassumption.
+    eapply root_no_pred'. eassumption.
     unfold is_effect_on.
     exists i, i', s, s'. 
     assumption.
@@ -444,13 +274,7 @@ Module Evaluation.
       rewrite <-nlcons_to_list in Hpre. eapply prefix_cons_cons in Hpre.      
       eapply in_prefix_in; eauto.
   Qed.
-(*
-  Lemma precedes_incl k t c c' :
-    Precedes k t c c' -> exists t', Precedes c' t' c c'.
-  Proof.
-    intros. dependent induction t; inv_tr H; eauto.
-  Qed.
-*)
+
   Lemma in_exists_pred p i s k (t : trace) :
     In (p, i, s) (k :<: `t) ->
     eff (ne_front (`t)) = Some k ->
@@ -459,7 +283,6 @@ Module Evaluation.
   Proof.
     intros H Heff Hneq.
     destruct t as [l tr]; cbn in H, Heff. unfold "`".
-      (*revert dependent p; revert dependent i; revert dependent s;*)
     destruct H; [subst k| revert dependent k];
       dependent induction l; inversion tr; subst; intros. 
     - exists root, start_tag, s0. split; [ constructor | eauto ]; eauto.
@@ -488,7 +311,7 @@ Module Evaluation.
     destruct t as [l tr]. induction l; inversion tr; subst; cbn in *; intros i Hin.
     - destruct Hin as [Hin|Hin]; [inversion Hin; eauto|contradiction].
     - destruct Hin.
-      + exfalso. destruct (ne_front l) as [[q j] r]. eapply root_no_pred. subst a.
+      + exfalso. destruct (ne_front l) as [[q j] r]. eapply root_no_pred'. subst a.
         apply edge_spec. unfold is_effect_on. exists j,i,r,s. eapply H2.
       + eapply IHl; eauto.
   Qed.
@@ -528,13 +351,6 @@ Module Evaluation.
       + cbn in *. subst a. destruct Hin; [inversion H3; reflexivity|].
         trace_proj t'. eapply ivec_fresh in H2; eauto. contradiction.
   Qed.
-
-(*  Lemma precedes_succ k t :
-    forall q j r q' j' r' p i s k' step, Precedes k t (q', j', r') (q, j, r) ->
-                                         eff (q, j, r) = Some (p, i, s) ->
-                                         p =/= q' ->
-                                         Precedes k' (Step k' k t step) (q', j', r') (p, i, s).
- *)
 
   Lemma ne_to_list_inj {A : Type} (l l' : ne_list A) :
     ne_to_list l = ne_to_list l' -> l = l'.
@@ -594,7 +410,6 @@ Module Evaluation.
     - econstructor; cbn; eauto.
       rewrite <-nlcons_to_list. eauto.
   Qed.
-
   
   Lemma precedes_step l q j r p i s :
     forall k, In (q, j, r) l ->
@@ -661,219 +476,7 @@ Module Evaluation.
       rewrite H in H1.
       inversion H1.
   Qed.
-(*
-    
-  Definition lab_tag_matches (l : Lab) (j : Tag) (k : Conf) : bool :=
-    match k with
-    | ((p, i), s) => (j ==b i) && (l ==b p) 
-    end.
-
-  Fixpoint label_tag_in_trace (l : Lab) (i : Tag) (k : Conf) (t : Tr k) : bool :=
-    match t with
-    | (Init s) => lab_tag_matches l i (root, start_tag, s)
-    | (Step k' k t _) => (lab_tag_matches l i k') || (label_tag_in_trace l i k t)
-    end.
-
-  Fixpoint label_in_trace (l : Lab) (k : Conf) (t : Tr k) : bool :=
-    match t with
-    | (Init s) => l ==b root
-    | (Step k' k t _) => (l ==b lab_of k') || (label_in_trace l k t)
-    end.
-
-  Lemma last_inst_self a l u t :
-     last_inst_of a (a, l, u) t = Some l.
-  Proof.
-    dependent induction t.
-    + simpl. destruct (root == root); firstorder. 
-    + simpl. destruct (a == a); firstorder. 
-  Qed.
-
-  Lemma last_inst_step l p i s k t step : 
-    l =/= p -> last_inst_of l k t = last_inst_of l (p, i, s) (Step (p, i, s) k t step).
-  Proof.
-    intros Hneq.
-    simpl. destruct (l == p); firstorder. 
-  Qed.
-    
-  Lemma last_inst_not_exists :
-    forall l k t, last_inst_of l k t = None <-> ~ exists i s, In k t (l, i, s).
-  Proof.
-    intros.
-    destruct k as [[p i] s].
-    dependent induction t.
-    + split; intros.
-      - simpl in H. destruct (l == root); try inversion H.
-        intro. destruct H0 as [j [r H0]].
-        inv_tr H0. contradiction c. reflexivity.
-      - simpl. destruct (l == root); try firstorder.
-        exfalso. rewrite e in *. eapply H. exists s. constructor.
-    + destruct k' as [[q j] r].
-      split; intros.
-      - simpl in H. destruct (l == p); [ inversion H |].
-        intro. eapply IHt; eauto.
-        destruct H0 as [m [w H0]]. exists m, w.
-        inv_tr H0; firstorder.
-      - simpl.
-        destruct (l == p).
-        * exfalso. apply H. rewrite e0. eauto using In.
-        * eapply IHt; eauto. intro. apply H.
-          destruct H0 as [m [w H0]].
-          eauto using In.
-  Qed.
-
-  Lemma last_inst_in :
-    forall l k t i, last_inst_of l k t = Some i -> exists s, In k t (l, i, s).
-  Proof.
-    intros. dependent induction t; simpl in H.
-    + destruct (l == root). 
-      - rewrite e in *. simpl in H. inversion H; subst. eexists. constructor.
-      - inversion H.
-    + destruct k as [[q j] r].
-      destruct (l == q).
-      - rewrite e0 in *. inversion H; subst. eexists. constructor.
-      - edestruct IHt; eauto. exists x. constructor. eassumption.
-  Qed.
   
-  Lemma last_inst_in_inv :
-    forall k t l i s, In k t (l, i, s) -> exists j, last_inst_of l k t = Some j.
-  Proof.
-    intros. dependent induction t; simpl in H.
-    + destruct (l == root). 
-      - rewrite e in *. simpl. exists start_tag. destruct (root == root); firstorder.
-      - inv_tr H. firstorder.
-    + destruct k as [[q j] r].
-      destruct (l == q).
-      - rewrite e0 in *. simpl. exists j. destruct (q == q); firstorder.
-      - inv_tr H.
-        * firstorder.
-        * eapply IHt in H4. destruct H4 as [j' Hlast].
-          eexists. simpl. destruct (l == q).
-          ** contradiction c. 
-          ** eapply Hlast.
-  Qed.
-
-  Lemma precedes_same p m s w t :
-    Precedes (p, m, s) t (p, m, w) (p, m, s) -> w === s.
-  Proof.
-    intros H.
-    eapply precedes_implies_in_pred in H.
-    inv_tr H; try reflexivity. 
-    exfalso. eapply ivec_fresh; eauto.
-  Qed.
-
-  Lemma in_same_state p i s s' t :
-    In (p, i, s) t (p, i, s') -> s === s'.
-  Proof.
-    intros.
-    inv_tr H; try reflexivity.
-    + inv_tr H. reflexivity.
-      exfalso. eapply ivec_fresh; eauto.
-  Qed.
-
-    Lemma last_inst_step_pred p j r a l u t e : 
-    a =/= p -> last_inst_of a (p, j, r) (Step (p, j, r) (a, l, u) t e) = Some l.
-  Proof.
-    intros Hneq.
-    simpl.
-    destruct (a == p); firstorder. eapply last_inst_self.
-  Qed.
-
-  Lemma label_in_trace_in :
-    forall l k t, label_in_trace l k t = true <-> exists i s, In k t (l, i, s).
-  Proof.
-    intros.
-    induction t.
-    - simpl. split; intros.
-      + exists start_tag, s. conv_bool. rewrite H. constructor.
-      + destruct H as [i [s' Hin]].
-        inv_tr Hin.
-        unfold equiv_decb.
-        destruct (root == root); destruct (start_tag == start_tag); firstorder.
-    - destruct k as [[p j] s].
-      split; intros.
-      + destruct (l == p).
-        * rewrite e0 in *. exists j, s. constructor.
-        * destruct IHt as [IHt _].
-          simpl in H. conv_bool.
-          destruct H; [ exfalso; firstorder |].
-          destruct IHt as [r [s' Hin]]; eauto.
-          exists r, s'. eauto using In.
-      + destruct IHt as [_ IHt].
-        destruct H as [r [s' Hin]].
-        simpl.
-        inv_tr Hin; unfold equiv_decb.
-        * destruct (l == l); firstorder.
-        * destruct (l == p); simpl; auto; eapply IHt; eauto.
-  Qed.
-
-  Lemma not_label_in_trace_in :
-    forall l k t, label_in_trace l k t = false <-> ~ exists i s, In k t (l, i, s).
-  Proof.
-    intros.
-    split; intros. intro.
-    + rewrite <- negb_true_iff in H.
-      apply Is_true_eq_left in H.
-      apply negb_prop_elim in H.
-      apply H.
-      apply Is_true_eq_left.
-      apply label_in_trace_in; assumption.
-    + rewrite <- negb_true_iff.
-      apply Is_true_eq_true.
-      apply negb_prop_intro.
-      intro. apply H.
-      apply Is_true_eq_true in H0.
-      apply label_in_trace_in; assumption.
-  Qed.
-
-  Lemma label_tag_in_trace_in :
-    forall l i k t, label_tag_in_trace l i k t = true <-> exists s, In k t (l, i, s).
-  Proof.
-    intros.
-    induction t.
-    - simpl. split; intros.
-      + exists s. conv_bool. destruct H. rewrite H. rewrite H0. constructor.
-      + destruct H as [s' Hin].
-        inv_tr Hin.
-        unfold equiv_decb.
-        destruct (root == root); destruct (start_tag == start_tag); firstorder.
-    - destruct k as [[p j] s].
-      split; intros.
-      remember (lab_tag_matches l i (p, j, s)) as eq.
-      symmetry in Heqeq. simpl in Heqeq.
-      + destruct eq; conv_bool.
-        * destruct Heqeq. rewrite H0. rewrite H1. exists s. constructor.
-        * destruct IHt as [IHt _].
-          simpl in H. conv_bool.
-          destruct H; [ exfalso; firstorder |].
-          destruct IHt as [r Hin]; eauto.
-          exists r. eauto using In.
-      + destruct IHt as [_ IHt].
-        destruct H as [r Hin].
-        simpl.
-        inv_tr Hin; unfold equiv_decb.
-        * destruct (l == l); destruct (i == i); firstorder.
-        * destruct (l == p); destruct (i == j); simpl; auto; eapply IHt; eauto.
-  Qed.
-
-  Lemma not_label_tag_in_trace_in :
-    forall l i k t, label_tag_in_trace l i k t = false <-> ~ exists s, In k t (l, i, s).
-  Proof.
-    intros.
-    split; intros. intro.
-    + rewrite <- negb_true_iff in H.
-      apply Is_true_eq_left in H.
-      apply negb_prop_elim in H.
-      apply H.
-      apply Is_true_eq_left.
-      apply label_tag_in_trace_in; assumption.
-    + rewrite <- negb_true_iff.
-      apply Is_true_eq_true.
-      apply negb_prop_intro.
-      intro. apply H.
-      apply Is_true_eq_true in H0.
-      apply label_tag_in_trace_in; assumption.
-  Qed.
-*)
   Definition lift (tr : Traces) : Hyper :=
     fun ts => ts = tr.
 
